LeanALaCarte/MergeModMaps.lean
@@ -19,7 +19,7 @@ def throwNotSameShape (e₁ e₂ : Expr) : CoreM α :=
 -- For now, the algorithm is really naive and merges exprs 2 by 2. Once this is stable and works well enough, we can optimise this function to take an array of exprs instead, and match on the first one.
 partial def mergeExprsBin (e₁ e₂ : Expr) : ModularM Expr :=
   withIncRecDepth do
-  e₁.withApp fun fn₁ args₁ => do
+  withTraceNode `Modular.MergeExprs (λ exn => withModMappedLCtx do return m!"mergeExprsBin {indentExpr e₁} {indentExpr e₂} \n⇒{← (return exn.toOption.map indentExpr)}") do  e₁.withApp fun fn₁ args₁ => do
   e₂.withApp fun fn₂ args₂ => do
   match fn₁,fn₂ with
   | .mvar m₁, .mvar m₂ => do
@@ -33,23 +33,26 @@ partial def mergeExprsBin (e₁ e₂ : Expr) : ModularM Expr :=
     let some matchers₂ := exts.get? m₂
       | trace[Modular.MergeExprs] "{Expr.mvar m₂} is not a matcher"
         return (mkAppN fn₁ args)
-    trace[Modular.MergeExprs] "Merging matchers {matchers₁.map (·.matchName)} and {matchers₂.map (·.matchName)}"
-    modifyMatchExtensions (· |>.erase m₁ |>.insert m₂ (matchers₁ ++ matchers₂))
+    trace[Modular.MergeExprs] "Merging matchers {matchers₁.map fun {matchName, mvar,..} => (matchName,Expr.mvar mvar)} and {matchers₂.map fun {matchName, mvar,..} => (matchName,Expr.mvar mvar)}}"
+    modifyMatchExtensions (· |>.erase m₂ |>.insert m₁ (matchers₁ ++ matchers₂))
     return (mkAppN fn₁ args)
-  | .mvar m₁, _  => do
-      let (_,n₁) ← getDelayedMVarRoot' m₁
-      let n₂ := args₁.size - n₁
-      assert! n₂ >= args₂.size
-      let args ← mergeArgs args₁[n₁:] args₂[:n₂]
-      let res := mkAppN fn₂ args
-      return res
-  | _,.mvar m₂  => do
-      let (_,n₂) ← getDelayedMVarRoot' m₂
-      let n₁ := args₂.size - n₂
-      assert! n₁ >= args₁.size
-      let args ← mergeArgs args₁[n₁:] args₂[:n₂]
-      let res := mkAppN fn₁ args
-      return res
+  | .mvar _, _  =>
+    return e₂
+      -- let (_,n₁) ← getDelayedMVarRoot' m₁
+      -- trace[Modular.MergeExprs] "number of delayed-assign args:"
+      -- let n₂ := args₁.size - n₁
+      -- assert! n₂ >= args₂.size
+      -- let args ← mergeArgs args₁[n₁:] args₂[:n₂]
+      -- let res := mkAppN fn₂ args
+      -- return res
+  | _,.mvar _  =>
+    return e₁
+      -- let (_,n₂) ← getDelayedMVarRoot' m₂
+      -- let n₁ := args₂.size - n₂
+      -- assert! n₁ >= args₁.size
+      -- let args ← mergeArgs args₁[n₁:] args₂[:n₂]
+      -- let res := mkAppN fn₁ args
+      -- return res
   | _,_ => return mkAppN (← traverse fn₁ fn₂) (← mergeArgs args₁ args₂)
 
 where
