LeanALaCarteTest/Merge.lean
@@ -1,0 +1,30 @@
+import LeanALaCarte
+
+inductive A where
+  | a : A → A
+
+def A.sizeOf : A → Nat
+  | a x => x.sizeOf + 1
+
+modular (name := `B)
+  inductive B extends A where
+    | b : B
+
+  mod def B.sizeOf extends A.sizeOf where
+    matcher match_1 with
+      | .b => 0
+
+modular (name := `C)
+  inductive C extends A where
+    | c : C → C → C
+
+  mod def C.sizeOf extends A.sizeOf where
+    matcher match_1 with
+      | .c x y => x.sizeOf + y.sizeOf + 1
+
+set_option trace.Modular true
+modular (imports := #[`B,`C])
+
+  inductive D extends B,C where
+
+  mod def D.sizeOf extends B.sizeOf, C.sizeOf
